Rewrite [remove_element]

DListRef.fst
@@ -438,46 +438,40 @@ let dlisthead_remove_tail #t h =
 #reset-options
 
 // TODO: See if possible to do without the StrongExcludedMiddle
-let rec get_ref_index (#t:Type) (s:seq (gpointer t)) (x:ref t{s `contains_by_addr` x}) :
-  GTot (i:nat{i < Seq.length s})
-    (decreases (Seq.length s)) =
-  let l = seq_to_list s in
+val remove_element_aux :
+  #t:Type ->
+  s:seq (gpointer t) ->
+  x:ref t{s `contains_by_addr` x} ->
+  GTot (idx:nat{idx < length s} & r:seq (gpointer t){
+      length r = length s - 1 /\
+      g_ptr_eq s.[idx] x /\
+      (forall (i:nat{i < length s}). (* {:pattern TODO} *) (
+                (i < idx ==> s.[i] == r.[i]) /\
+                (i > idx ==> s.[i] == r.[i-1])))})
+    (decreases (length s))
+let rec remove_element_aux #t s x =
   contains_elim s x;
   let h, t = Seq.head s, Seq.tail s in
-  if FStar.StrongExcludedMiddle.strong_excluded_middle (g_ptr_eq h x) then 0 else (
+  if StrongExcludedMiddle.strong_excluded_middle (g_ptr_eq h x) then (|0, t|) else (
     contains_cons h t x;
-    1 + get_ref_index t x)
+    let (|idx, r|) = remove_element_aux t x in
+    (|idx + 1, Seq.cons h r |))
 
-val lemma_get_ref_index : #t:Type -> s:seq (gpointer t) -> x:ref t{s `contains_by_addr` x} ->
-  Lemma (ensures (
-    g_ptr_eq s.[get_ref_index s x] x))
-    (decreases (Seq.length s))
-    [SMTPat (g_ptr_eq s.[get_ref_index s x] x)]
-let rec lemma_get_ref_index #t s x =
-  contains_elim s x;
-  let h, t = Seq.head s, Seq.tail s in
-  if FStar.StrongExcludedMiddle.strong_excluded_middle (g_ptr_eq h x) then () else (
-    contains_cons h t x;
-    lemma_get_ref_index t x)
-
-val split_seq_at_element : #t:Type -> s:seq (gpointer t) -> x:ref t{s `contains_by_addr` x} ->
-  GTot (v:(seq (ref t) * nat * seq (ref t)){
-      let l, i, r = v in
-      indexable s i /\ (
-      let (i:nat{i < length s}) = i in // workaround for two phase thing
-      s == append l (cons s.[i] r) /\
-      g_ptr_eq s.[i] x)
-  })
-let split_seq_at_element #t s x =
-  let i = get_ref_index s x in
-  let l, mr = Seq.split s i in
-  lemma_split s i;
-  l, i, tail mr
-
-unfold let remove_element (#t:Type) (s:seq (gpointer t)) (x:ref t{s `contains_by_addr` x}) :
-  GTot (seq (gpointer t)) =
-  let l, i, r = split_seq_at_element s x in
-  Seq.append l r
+irreducible
+val remove_element :
+  #t:Type ->
+  s:seq (gpointer t) ->
+  x:ref t{s `contains_by_addr` x} ->
+  GTot (r:seq (gpointer t){
+      (exists (idx:nat{idx < length s}).
+          length r = length s - 1 /\
+          g_ptr_eq s.[idx] x /\
+          (forall (i:nat{i < length s}). (* {:pattern TODO} *) (
+                    (i < idx ==> s.[i] == r.[i]) /\
+                    (i > idx ==> s.[i] == r.[i-1]))))})
+    (decreases (length s))
+let rec remove_element #t s x =
+  dsnd (remove_element_aux s x)
 
 #reset-options "--z3rlimit 1 --detail_errors --z3rlimit_factor 20"
 
